---
date: 2024-03-21 12:31
tags:
  - newNotes
  - math
  - notes
---
Links: [[Math MOC]]

---
# Rational Function
$R(x)=\frac{polynomial}{polynomail}$

## Ex:
$f(x)=\frac{x-1}{x+2}$
![[Pasted image 20240321123537.png|560]]

x- and y-intercepts
## x-intercept
$y=0$ Solve for x

## y-intercept
$x=0$ Solve for y

$0=\frac{x-1}{x+2}$
$0=x-1$
$1=x$

$y=\frac{0-1}{0+2}=\frac{1}{2}$
$y=-\frac{1}{2}$ 

# Vertical Asymptotes
$x+2=0$
V.A - $x=-2$
# Horizontal Asymptotes
- Highest degree in the numerator = $n$
- Highest degree in the denominator = $m$
$n=1$
$m=1$
## Case 1
$n > m$ No H.A
## Case 2
$n<m$ x-axis($y=0$) H.A
## Case 3
$n=m$ $y=\frac{a}{b}$
- Where $a$ is coefficient of the highest power in the numerator
- $b$ is coefficient of the highest power in the denominator
$y=\frac{1x^{1(a)}-1}{1x^{1(b)}+2}$
# Graph
X-Int = $x=1$
Y-Int = $y=-\frac{1}{2}$
V.A = $x=-2$
H.A = $y=1$
![[Pasted image 20240321125208.png|560]]
# Ex:
$f(x)=\frac{x+1}{(x-3)(x+2)}$

$y=\frac{x-1}{(x-3)(x+2)}$
$y=\frac{0+1}{(0-3)(0+2)}=\frac{1}{(-3)(2)}=\frac{1}{-6}=-\frac{1}{6}$
$y=-\frac{1}{6}$

$0=x+1$
$-1=x$

$(x-3)(x+2)=0$
$\begin{matrix}x-3=0 & x+2=0 \\ x=3 & x=-2\end{matrix}$ 
$f(x)=\frac{1x^1}{1x^2-1x-6}$
$n=1$
$m=2$
$n<m=x-axis$
![[Pasted image 20240321130951.png|560]]
$x=-3$
$f(-3)=\frac{-3+1}{(-3-3)(-3+2)}=\frac{-2}{(-6)(-1)}=\frac{-6}{-1}=\frac{-2}{6}+(-\frac{1}{3})$



---
