---
date: 2024-03-26 12:32:52
tags:
  - newNotes
---

Links: 

---
# Notes
$f(x)=\frac{x-3}{2x^{2}+3x-2}$
$\begin{align}x&=3 \\ y&=\frac{3}{2}\end{align}$

$\begin{align}x&=\frac{-3±\sqrt{3^{2}-4(2)(-2)}}{2(2)} \\ &=\frac{-3±\sqrt{9+16}}{4}\end{align}$
$\begin{matrix}\begin{align}x&=\frac{-3+5}{4} & x&=\frac{-3-5}{4}  \\ x&=\frac{2}{4}=\frac{1}{2} & x&=-\frac{8}{4}=-2\end{align}\end{matrix}$
H.A= x-axis
![[Pasted image 20240326124849.png|560]]
f(2)=-
f(0)=+
f(4)=+
f(-3)=-

# Example
$C(t)=\frac{t}{t^{2}+1}$
What will happen to $C(t)$ as $t\frac{\rightarrow}{approaches}\infty$?

# Exponential Function
$f(x)=2^{x}$


---
